More progress on sha_final proof

progs/verif_sha_final.v
@@ -19,12 +19,52 @@ Proof. intros.
   repeat  rewrite align_1. rewrite Z.mul_1_l. auto.
 Qed.
 
-Lemma Zlength_zeros: forall n, Zlength (zeros n) = n.
-Admitted.
+Lemma Zlength_zeros: 
+    forall n, (n>=0)%Z -> Zlength (zeros n) = n.
+Proof.
+intros.
+rewrite <- (Z2Nat.id n) in * by omega.
+clear H.
+induction (Z.to_nat n).
+reflexivity.
+rewrite inj_S.
+rewrite zeros_equation.
+pose proof (Zgt_cases (Z.succ (Z.of_nat n0)) 0).
+destruct (Z.succ (Z.of_nat n0) >? 0); try omega.
+rewrite Zlength_cons.
+f_equal.  rewrite <- IHn0.
+f_equal. f_equal. omega.
+Qed.
 
 Lemma nth_map_zeros:
  forall i j v, (Z.of_nat i < j)%Z -> nth i (map Vint (zeros j)) v = Vint Int.zero.
-Admitted.
+Proof.
+intros.
+rewrite <- (Z2Nat.id j) in * by omega.
+apply Nat2Z.inj_lt in H.
+replace (Z.to_nat j) with (Z.to_nat j - S i + S i) by omega.
+forget (Z.to_nat j - S i) as k.
+clear j H.
+rewrite Nat2Z.inj_add.
+rewrite inj_S.
+induction i.
+rewrite zeros_equation.
+pose proof (Zgt_cases (Z.of_nat k + Z.succ (Z.of_nat 0)) 0).
+destruct (Z.of_nat k + Z.succ (Z.of_nat 0) >? 0); try omega.
+simpl. reflexivity.
+rewrite zeros_equation.
+pose proof (Zgt_cases (Z.of_nat k + Z.succ (Z.of_nat (S i))) 0).
+destruct (Z.of_nat k + Z.succ (Z.of_nat (S i)) >? 0); try omega.
+rewrite map_cons.
+unfold nth.
+rewrite <- IHi.
+unfold nth.
+f_equal.
+f_equal.
+f_equal.
+rewrite inj_S.
+omega.
+Qed.
 
 Hint Rewrite eval_var_env_set : norm. (* needed? *)
 
@@ -52,11 +92,11 @@ repeat rewrite Int.unsigned_repr in H2 by assumption.
 auto.
 Qed.
 
-Lemma length_zeros: forall n, length (zeros n) = Z.to_nat n.
+Lemma length_zeros: forall n,  (n >= 0)%Z -> length (zeros n) = Z.to_nat n.
 Proof.
-intros. pose proof (Zlength_zeros n).
-rewrite Zlength_correct in H.
-rewrite <- H at 2.
+intros. pose proof (Zlength_zeros n H). 
+rewrite Zlength_correct in H0.
+rewrite <- H0 at 2.
 rewrite Nat2Z.id. auto.
 Qed.
 
@@ -302,6 +342,7 @@ rewrite Zlength_cons; rewrite Zlength_nil.
 unfold ddlen.
 change (LBLOCK*4)%nat with CBLOCK.
 clear; omega.
+ change (Z.of_nat CBLOCK) with 64%Z; omega.
  forward. (* sha256_block_data_order (c,p); *)
  match goal with H : True |- _ => clear H 
             (* WARNING__ is a bit over-eager;
@@ -352,6 +393,7 @@ rewrite length_zeros.
 apply Nat2Z.inj_lt.
 rewrite Z2Nat.id by omega. 
 change (Z.of_nat 8) with 8%Z. omega.
+omega.
 entailer!.
 * change CBLOCK with 64; clear; omega.
 * apply divide_length_app.
@@ -377,6 +419,727 @@ entailer!.
  rewrite Zlength_correct; rewrite length_intlist_to_Zlist.
  rewrite map_length; rewrite H1.
  reflexivity.
+Qed.
+
+Lemma ltu_repr_false: forall i j, 
+ (0 <= i <= Int.max_unsigned -> 
+  0 <= j <= Int.max_unsigned -> 
+  Int.ltu (Int.repr i) (Int.repr j) = false -> i>=j)%Z.
+Proof.
+intros. unfold Int.ltu in H1. if_tac in H1; inv H1.
+repeat rewrite Int.unsigned_repr in H2 by assumption.
+auto.
+Qed.
+
+Definition final_loop :=
+ (Ssequence (Sset _xn (Econst_int (Int.repr 0) tint))
+                 (Sloop
+                    (Ssequence
+                       (Sifthenelse
+                          (Ebinop Olt (Etempvar _xn tuint)
+                             (Ebinop Odiv (Econst_int (Int.repr 32) tint)
+                                (Econst_int (Int.repr 4) tint) tint) tint)
+                          Sskip Sbreak)
+                       (Ssequence
+                          (Sset _ll
+                             (Ederef
+                                (Ebinop Oadd
+                                   (Efield
+                                      (Ederef
+                                         (Etempvar _c
+                                            (tptr t_struct_SHA256state_st))
+                                         t_struct_SHA256state_st) _h
+                                      (tarray tuint 8)) (Etempvar _xn tuint)
+                                   (tptr tuint)) tuint))
+                          (Ssequence
+                             (Scall None
+                                (Evar ___builtin_write32_reversed
+                                   (Tfunction
+                                      (Tcons (tptr tuint) (Tcons tuint Tnil))
+                                      tvoid))
+                                [Ecast (Etempvar _md (tptr tuchar))
+                                   (tptr tuint), Etempvar _ll tuint])
+                             (Sset _md
+                                (Ebinop Oadd (Etempvar _md (tptr tuchar))
+                                   (Econst_int (Int.repr 4) tint)
+                                   (tptr tuchar))))))
+                    (Sset _xn
+                       (Ebinop Oadd (Etempvar _xn tuint)
+                          (Econst_int (Int.repr 1) tint) tuint)))).
+
+Lemma lastblock_lemma:
+  forall (hi lo : int) (pad : Z) (hashed dd hashed' dd' : list int),
+length (map Int.unsigned dd') + 8 <= CBLOCK ->
+(0 <= pad < 8)%Z ->
+NPeano.divide LBLOCK (length hashed') ->
+length dd < CBLOCK ->
+NPeano.divide LBLOCK (length hashed) ->
+intlist_to_Zlist (map swap hashed') ++ map Int.unsigned dd' =
+intlist_to_Zlist (map swap hashed) ++
+map Int.unsigned dd ++ [128%Z] ++ map Int.unsigned (zeros pad) ->
+(Zlength hashed * 4 + Zlength dd)%Z = hilo hi lo ->
+map Int.repr
+  (intlist_to_Zlist
+     (map swap
+        (list_drop (length hashed')
+           (generate_and_pad
+              (intlist_to_Zlist (map swap hashed) ++ map Int.unsigned dd) 0)))) =
+dd' ++
+zeros (Z.of_nat CBLOCK - 8 - Zlength dd') ++
+map Int.repr (intlist_to_Zlist (map swap [hi, lo])).
+Proof.
+intros.
+Admitted.
+
+Lemma nth_map':
+  forall {A B} (f: A -> B) d d' i al,
+  i < length al ->
+   nth i (map f al) d = f (nth i al d').
+Proof.
+induction i; destruct al; simpl; intros; try omega; auto.
+apply IHi; omega.
+Qed.
+
+
+Lemma array_at_ZnthV_nil:
+  forall t sh, array_at t sh (ZnthV t nil) = array_at_ t sh.
+Proof. intros.
+unfold array_at_.
+extensionality lo hi.
+apply array_at_ext; intros.
+unfold ZnthV. if_tac; auto. rewrite nth_overflow; auto.
+simpl; omega.
+Qed.
+
+Lemma final_part4:
+ forall (Espec: OracleKind) md c shmd hashedmsg,
+semax
+  (initialized _ignore'2
+     (initialized _cNl
+        (initialized _cNh
+           (initialized _ignore (initialized _ignore'1 Delta_final_if1)))))
+  (PROP  ()
+   LOCAL  (`(eq md) (eval_id _md); `(eq c) (eval_id _c))
+   SEP 
+   (`(array_at tuchar Tsh (fun _ : Z => Vint Int.zero) 0 64
+        (offset_val (Int.repr 40) c));
+   `(array_at tuint Tsh (tuints hashedmsg) 0 8 c); K_vector;
+   `(field_at_ Tsh t_struct_SHA256state_st _Nl c);
+   `(field_at_ Tsh t_struct_SHA256state_st _Nh c);
+   `(field_at Tsh t_struct_SHA256state_st _num (Vint (Int.repr 0)) c);
+   `(memory_block shmd (Int.repr 32) md)))
+  (Ssequence final_loop (Sreturn None))
+  (function_body_ret_assert tvoid
+     (PROP  ()
+      LOCAL ()
+      SEP  (K_vector; `(data_at_ Tsh t_struct_SHA256state_st c);
+      `(data_block shmd (intlist_to_Zlist hashedmsg) md)))).
+Admitted.
+
+Lemma sha_final_part3:
+forall (Espec : OracleKind) (md c : val) (shmd : share) (hi lo : int)
+  (dd hashed hashed' dd' : list int) (pad : Z),
+(Zlength hashed * 4 + Zlength dd)%Z = hilo hi lo ->
+length dd < CBLOCK ->
+length (map Int.unsigned dd') + 8 <= CBLOCK ->
+(0 <= pad < 8)%Z ->
+NPeano.divide LBLOCK (length hashed') ->
+intlist_to_Zlist (map swap hashed') ++ map Int.unsigned dd' =
+intlist_to_Zlist (map swap hashed) ++
+map Int.unsigned dd ++ [128%Z] ++ map Int.unsigned (zeros pad) ->
+semax
+  (initialized _cNl
+     (initialized _cNh
+        (initialized _ignore (initialized _ignore'1 Delta_final_if1))))
+  (PROP  ()
+   LOCAL  (`(eq (offset_val (Int.repr 40) c)) (eval_id _p);
+   `(eq (Vint lo)) (eval_id _cNl); `(eq (Vint hi)) (eval_id _cNh);
+   `(eq (Vint (Int.repr (Zlength dd')))) (eval_id _n);
+   `(eq md) (eval_id _md); `(eq c) (eval_id _c))
+   SEP 
+   (`(data_block Tsh
+        (intlist_to_Zlist
+           (map swap
+              (list_drop (length hashed')
+                 (generate_and_pad
+                    (intlist_to_Zlist (map swap hashed) ++
+                     map Int.unsigned dd) 0)))) (offset_val (Int.repr 40) c));
+   `(array_at tuint Tsh
+       (ZnthV tuint (map Vint (process_msg init_registers hashed'))) 0 8 c);
+   `(field_at_ Tsh t_struct_SHA256state_st _Nl c);
+   `(field_at_ Tsh t_struct_SHA256state_st _Nh c);
+   `(field_at_ Tsh t_struct_SHA256state_st _num c); K_vector;
+   `(memory_block shmd (Int.repr 32) md)))
+  (Ssequence
+     (Scall None
+        (Evar _sha256_block_data_order
+           (Tfunction
+              (Tcons (tptr t_struct_SHA256state_st) (Tcons (tptr tvoid) Tnil))
+              tvoid))
+        [Etempvar _c (tptr t_struct_SHA256state_st),
+        Etempvar _p (tptr tuchar)])
+     (Ssequence
+        (Sassign
+           (Efield
+              (Ederef (Etempvar _c (tptr t_struct_SHA256state_st))
+                 t_struct_SHA256state_st) _num tuint)
+           (Econst_int (Int.repr 0) tint))
+        (Ssequence
+           (Ssequence
+              (Scall (Some _ignore'2)
+                 (Evar _memset
+                    (Tfunction
+                       (Tcons (tptr tvoid) (Tcons tint (Tcons tuint Tnil)))
+                       (tptr tvoid)))
+                 [Etempvar _p (tptr tuchar), Econst_int (Int.repr 0) tint,
+                 Ebinop Omul (Econst_int (Int.repr 16) tint)
+                   (Econst_int (Int.repr 4) tint) tint])
+              (Sset _ignore (Etempvar _ignore'2 (tptr tvoid))))
+           (Ssequence final_loop (Sreturn None)))))
+  (function_body_ret_assert tvoid
+     (PROP  ()
+      LOCAL ()
+      SEP  (K_vector; `(data_at_ Tsh t_struct_SHA256state_st c);
+      `(data_block shmd
+          (intlist_to_Zlist
+             (process_msg init_registers
+                (generate_and_pad_msg
+                   (intlist_to_Zlist (map swap hashed) ++ map Int.unsigned dd))))
+          md)))).
+Proof.
+intros.
+assert (LD: length
+  (list_drop (length hashed')
+     (generate_and_pad
+        (intlist_to_Zlist (map swap hashed) ++ map Int.unsigned dd) 0)) =
+    LBLOCK).
+admit.  (* looks fine *)
+forward. (* sha256_block_data_order (c,p); *)
+(*  hashed: list int, b: list int, ctx : val, data: val, sh: share *)
+instantiate (1:= (hashed',
+           (list_drop (length hashed')
+              (generate_and_pad
+                 (intlist_to_Zlist (map swap hashed) ++ map Int.unsigned dd)
+                 0)),
+        c, (offset_val (Int.repr 40) c), Tsh))
+  in (Value of witness).
+entailer!.
+unfold K_vector. normalize.
+ erewrite elim_globals_only by (split3; [eassumption | reflexivity.. ]).
+cancel.
+normalize.
+replace_SEP 0%Z  (`(array_at tuint Tsh
+          (tuints
+             (process_msg init_registers
+                (hashed' ++
+                 list_drop (length hashed')
+                   (generate_and_pad
+                      (intlist_to_Zlist (map swap hashed) ++
+                       map Int.unsigned dd) 0)))) 0 8 c) *
+      `(at_offset 40 (array_at tuchar Tsh (ZnthV tuchar []) 0 64) c) *
+      K_vector).
+entailer!.
+unfold K_vector. normalize.
+ erewrite elim_globals_only by (split3; [eassumption | reflexivity.. ]).
+cancel.
+unfold data_block.
+rewrite array_at_ZnthV_nil.
+rewrite Zlength_correct.
+rewrite length_intlist_to_Zlist.
+rewrite map_length. rewrite LD.
+change (Z.of_nat (4 * LBLOCK))%Z with 64%Z.
+unfold at_offset.
+apply array_at__array_at.
+normalize.
+replace (hashed' ++
+               list_drop (length hashed')
+                 (generate_and_pad
+                    (intlist_to_Zlist (map swap hashed) ++
+                     map Int.unsigned dd) 0))
+  with  (generate_and_pad_msg
+                    (intlist_to_Zlist (map swap hashed) ++
+                     map Int.unsigned dd)).
+Focus 2.
+admit.  (* looks fine *)
+forward. (* c->num=0; *)
+forward. (* ignore=memset (p,0,SHA_CBLOCK); *)
+instantiate (1:= (Tsh, (offset_val (Int.repr 40) c), 64%Z, Int.zero))
+  in (Value of witness).
+entailer!.
+change (Int.repr 64) with (Int.repr (sizeof (tarray tuchar 64))).
+rewrite memory_block_typed.
+simpl_data_at.
+pull_left (at_offset 40 (array_at tuchar Tsh (ZnthV tuchar []) 0 64) c).
+repeat rewrite sepcon_assoc; apply sepcon_derives; [ | cancel].
+unfold at_offset.
+cancel.
+reflexivity.
+autorewrite with subst.
+replace_SEP 0%Z (`(array_at tuchar Tsh (fun _ : Z => Vint Int.zero) 0 64
+          (offset_val (Int.repr 40) c))).
+entailer!.
+forward.  (* ignore = ignore'; *)
+fold t_struct_SHA256state_st.
+
+forget  (process_msg init_registers
+             (generate_and_pad_msg
+                (intlist_to_Zlist (map swap hashed) ++ map Int.unsigned dd)))
+  as hashedmsg.
+
+replace Delta with
+ (initialized _ignore'2 (initialized _cNl (initialized _cNh (initialized _ignore (initialized _ignore'1 Delta_final_if1)))))
+ by (simplify_Delta; reflexivity).
+eapply semax_pre; [ | apply final_part4].
+entailer!.
+Qed.
+
+Lemma final_part5:
+forall (hashed dd hashed' dd' : list int) (pad : Z) (hi' lo' : list Z)
+  (hi lo : int) c_,
+NPeano.divide LBLOCK (length hashed) ->
+length dd < CBLOCK ->
+(Zlength dd < 64)%Z ->
+length (map Int.unsigned dd') + 8 <= CBLOCK ->
+(0 <= pad < 8)%Z ->
+NPeano.divide LBLOCK (length hashed') ->
+intlist_to_Zlist (map swap hashed') ++ map Int.unsigned dd' =
+intlist_to_Zlist (map swap hashed) ++
+map Int.unsigned dd ++ [128%Z] ++ map Int.unsigned (zeros pad) ->
+length hi' = 4 ->
+length lo' = 4 ->
+(Zlength hashed * 4 + Zlength dd)%Z = hilo hi lo ->
+isptr c_ ->
+hi' = intlist_to_Zlist [swap hi] /\ lo' = intlist_to_Zlist [swap lo] ->
+array_at tuchar Tsh (ZnthV tuchar (map Vint (map Int.repr lo'))) 0 4
+  (offset_val (Int.repr 100) c_) *
+array_at tuchar Tsh (ZnthV tuchar (map Vint (map Int.repr hi'))) 0 4
+  (offset_val (Int.repr 96) c_) *
+array_at tuchar Tsh (fun _ : Z => Vint Int.zero) 0
+  (Z.of_nat CBLOCK - 8 - Zlength dd')
+  (offset_val (Int.repr (Zlength dd' + 40)) c_) *
+array_at tuchar Tsh (ZnthV tuchar (map Vint dd')) 0 (Zlength dd')
+  (offset_val (Int.repr 40) c_)
+|-- array_at tuchar Tsh
+      (ZnthV tuchar
+         (map Vint
+            (dd' ++
+             zeros (Z.of_nat CBLOCK - 8 - Zlength dd') ++
+             map Int.repr (hi' ++ lo')))) 0 64 (offset_val (Int.repr 40) c_).
+Proof.
+intros until c_.
+intros H4 H3 H3' H0 H1 H2 H5 Lhi Llo H7 Pc_ Hhilo.
+ rewrite (split_array_at (Zlength dd') tuchar Tsh _ 0 64)
+  by (clear - H0; rewrite Zlength_correct; change CBLOCK with 64 in H0;
+  rewrite map_length in H0; omega).
+ rewrite (split_array_at 56 tuchar Tsh _ (Zlength dd') 64)
+  by (clear - H0; rewrite Zlength_correct; change CBLOCK with 64 in H0;
+  rewrite map_length in H0; omega).
+ rewrite (split_array_at 60 tuchar Tsh _ 56 64) by omega.
+ replace (offset_val (Int.repr 100) c_) with
+            (offset_val (Int.repr (sizeof tuchar * 60)) (offset_val (Int.repr 40) c_))
+  by (rewrite offset_offset_val; destruct c_; reflexivity).
+ replace (offset_val (Int.repr 96) c_) with
+            (offset_val (Int.repr (sizeof tuchar * 56)) (offset_val (Int.repr 40) c_))
+  by (rewrite offset_offset_val; destruct c_; reflexivity).
+ replace (offset_val (Int.repr (Zlength dd' + 40)) c_) with
+            (offset_val (Int.repr (sizeof tuchar * Zlength dd')) (offset_val (Int.repr 40) c_))
+  by (change (sizeof tuchar) with 1%Z; rewrite Z.mul_1_l; rewrite offset_offset_val; rewrite Int.add_commut, add_repr; reflexivity).
+ forget (offset_val (Int.repr 40) c_) as cc.
+ repeat rewrite <- offset_val_array_at.
+ apply derives_trans with
+  (array_at tuchar Tsh (ZnthV tuchar (map Vint dd')) 0 (Zlength dd') cc *
+   array_at tuchar Tsh (fun _ : Z => Vint Int.zero) (Zlength dd' + 0)
+   (Zlength dd' + (Z.of_nat CBLOCK - 8 - Zlength dd')) cc *
+   array_at tuchar Tsh (fun i : Z => ZnthV tuchar (map Vint (map Int.repr hi')) (i - 56)) 
+      56 60 cc *
+  array_at tuchar Tsh (fun i : Z => ZnthV tuchar (map Vint (map Int.repr lo')) (i - 60)) 
+      60 64 cc);
+  [solve [cancel] | ].
+ rewrite Z.add_0_r.
+ replace (Zlength dd' + (Z.of_nat CBLOCK - 8 - Zlength dd'))%Z
+  with 56%Z by (change (Z.of_nat CBLOCK) with 64%Z; clear; omega).
+ assert (Zlength dd' >= 0)%Z by (rewrite Zlength_correct; omega).
+ assert (Zlength dd' = Z.of_nat (length (map Vint dd'))).
+ rewrite Zlength_correct, map_length; reflexivity.
+ assert (Z.of_nat CBLOCK - 8 - Z.of_nat (length dd') >= 0)%Z.
+    clear - H0; admit. (* tedious *)
+ repeat rewrite sepcon_assoc;
+ repeat apply sepcon_derives; apply derives_refl';
+ apply equal_f; try apply array_at_ext; intros;
+ unfold ZnthV; repeat rewrite if_false by omega.
++ repeat rewrite map_app.
+   rewrite app_nth1; [reflexivity | ].
+ apply Nat2Z.inj_lt. rewrite Z2Nat.id by omega; omega.
++ repeat rewrite map_app.
+   rewrite app_nth2. rewrite app_nth1.
+  rewrite nth_map_zeros. auto.
+  change (Z.of_nat CBLOCK) with 64%Z. 
+  rewrite Nat2Z.inj_sub.
+  rewrite Z2Nat.id by omega.
+  omega.
+  apply Nat2Z.inj_le.
+  rewrite Z2Nat.id by omega.
+  omega.
+  rewrite (map_length _ (zeros _)).
+  rewrite length_zeros.
+  change (Z.of_nat CBLOCK - 8)%Z with 56%Z.
+  apply Nat2Z.inj_lt.
+  rewrite Z2Nat.id by omega.
+  rewrite Nat2Z.inj_sub.
+  rewrite Z2Nat.id by omega.
+  omega.
+  apply Nat2Z.inj_le; try omega.
+  rewrite Z2Nat.id by omega.
+  omega.
+ change (Z.of_nat CBLOCK - 8)%Z with 56%Z; omega.
+  apply Nat2Z.inj_ge; try omega.
+  rewrite Z2Nat.id by omega.
+  omega.
++ repeat rewrite map_app.
+   rewrite <- app_ass.
+   rewrite app_nth2. rewrite app_nth1.
+   f_equal.
+   rewrite Z2Nat.inj_sub by omega.
+   f_equal.
+   rewrite app_length.
+   rewrite H6.
+  repeat rewrite map_length.
+  rewrite length_zeros.
+  change (Z.of_nat CBLOCK - 8)%Z with 56%Z.
+  rewrite Z2Nat.inj_sub; try omega.
+  rewrite Nat2Z.id; try omega.
+  assert (length dd' <= Z.to_nat 56); [ | omega].
+  rewrite map_length in H0; change CBLOCK with 64 in H0.
+  change (Z.to_nat 56) with 56; omega.
+  auto. 
+  rewrite app_length; rewrite (map_length _ (zeros _)); rewrite length_zeros.
+  rewrite H6. repeat rewrite map_length.
+  rewrite Lhi.
+    change (Z.of_nat CBLOCK - 8)%Z with 56%Z.
+  apply Nat2Z.inj_lt; try omega.
+  clear - H9; admit.  (* tedious *)
+  rewrite Zlength_correct; omega.
+  rewrite H6; repeat rewrite app_length; repeat rewrite map_length;
+   rewrite length_zeros.
+  clear - H9; admit.  (* tedious *)
+  auto.
++ admit.  (* tedious *)
+Qed.
+
+Lemma final_part2:
+forall (Espec : OracleKind) (hashed : list int) (md c : val) (shmd : share),
+writable_share shmd ->
+name _md ->
+name _c ->
+name _p ->
+name _n ->
+name _cNl ->
+name _cNh ->
+name _ignore ->
+forall (hi lo : int) (dd : list int),
+NPeano.divide LBLOCK (length hashed) ->
+(Zlength hashed * 4 + Zlength dd)%Z = hilo hi lo ->
+length dd < CBLOCK ->
+(Zlength dd < 64)%Z ->
+forall (hashed' dd' : list int) (pad : Z),
+length (map Int.unsigned dd') + 8 <= CBLOCK ->
+(0 <= pad < 8)%Z ->
+NPeano.divide LBLOCK (length hashed') ->
+intlist_to_Zlist (map swap hashed') ++ map Int.unsigned dd' =
+intlist_to_Zlist (map swap hashed) ++
+map Int.unsigned dd ++ [128%Z] ++ map Int.unsigned (zeros pad) ->
+forall p0 : val,
+semax (initialized _ignore (initialized _ignore'1 Delta_final_if1))
+  (PROP  ()
+   LOCAL 
+   (`(eq (force_val (sem_add_pi tuchar p0 (Vint (Int.repr (16 * 4 - 8))))))
+      (eval_id _p); `(eq (Vint (Int.repr (Zlength dd')))) (eval_id _n);
+   `(eq p0) (`(offset_val (Int.repr 40)) (`force_ptr (eval_id _c)));
+   `(eq md) (eval_id _md); `(eq c) (eval_id _c))
+   SEP 
+   (`(array_at tuchar Tsh (fun _ : Z => Vint Int.zero) 0
+        (Z.of_nat CBLOCK - 8 - Zlength dd')
+        (offset_val (Int.repr (40 + Zlength dd')) c));
+   `(array_at tuint Tsh
+       (ZnthV tuint (map Vint (process_msg init_registers hashed'))) 0 8 c);
+   `(field_at Tsh t_struct_SHA256state_st _Nl (Vint lo) c);
+   `(field_at Tsh t_struct_SHA256state_st _Nh (Vint hi) c);
+   `(array_at tuchar Tsh (ZnthV tuchar (map Vint dd')) 0 (Zlength dd')
+       (offset_val (Int.repr 40) c));
+   `(array_at tuchar Tsh (ZnthV tuchar (map Vint dd')) (Z.of_nat CBLOCK - 8)
+       64 (offset_val (Int.repr 40) c));
+   `(field_at_ Tsh t_struct_SHA256state_st _num c); K_vector;
+   `(memory_block shmd (Int.repr 32) md)))
+  (Ssequence
+     (Sset _cNh
+        (Efield
+           (Ederef (Etempvar _c (tptr t_struct_SHA256state_st))
+              t_struct_SHA256state_st) _Nh tuint))
+     (Ssequence
+        (Ssequence
+           (Scall None
+              (Evar ___builtin_write32_reversed
+                 (Tfunction (Tcons (tptr tuint) (Tcons tuint Tnil)) tvoid))
+              [Ecast (Etempvar _p (tptr tuchar)) (tptr tuint),
+              Etempvar _cNh tuint])
+           (Sset _p
+              (Ebinop Oadd (Etempvar _p (tptr tuchar))
+                 (Econst_int (Int.repr 4) tint) (tptr tuchar))))
+        (Ssequence
+           (Sset _cNl
+              (Efield
+                 (Ederef (Etempvar _c (tptr t_struct_SHA256state_st))
+                    t_struct_SHA256state_st) _Nl tuint))
+           (Ssequence
+              (Ssequence
+                 (Scall None
+                    (Evar ___builtin_write32_reversed
+                       (Tfunction (Tcons (tptr tuint) (Tcons tuint Tnil))
+                          tvoid))
+                    [Ecast (Etempvar _p (tptr tuchar)) (tptr tuint),
+                    Etempvar _cNl tuint])
+                 (Sset _p
+                    (Ebinop Oadd (Etempvar _p (tptr tuchar))
+                       (Econst_int (Int.repr 4) tint) (tptr tuchar))))
+              (Ssequence
+                 (Sset _p
+                    (Ebinop Osub (Etempvar _p (tptr tuchar))
+                       (Ebinop Omul (Econst_int (Int.repr 16) tint)
+                          (Econst_int (Int.repr 4) tint) tint) (tptr tuchar)))
+                 (Ssequence
+                    (Scall None
+                       (Evar _sha256_block_data_order
+                          (Tfunction
+                             (Tcons (tptr t_struct_SHA256state_st)
+                                (Tcons (tptr tvoid) Tnil)) tvoid))
+                       [Etempvar _c (tptr t_struct_SHA256state_st),
+                       Etempvar _p (tptr tuchar)])
+                    (Ssequence
+                       (Sassign
+                          (Efield
+                             (Ederef
+                                (Etempvar _c (tptr t_struct_SHA256state_st))
+                                t_struct_SHA256state_st) _num tuint)
+                          (Econst_int (Int.repr 0) tint))
+                       (Ssequence
+                          (Ssequence
+                             (Scall (Some _ignore'2)
+                                (Evar _memset
+                                   (Tfunction
+                                      (Tcons (tptr tvoid)
+                                         (Tcons tint (Tcons tuint Tnil)))
+                                      (tptr tvoid)))
+                                [Etempvar _p (tptr tuchar),
+                                Econst_int (Int.repr 0) tint,
+                                Ebinop Omul (Econst_int (Int.repr 16) tint)
+                                  (Econst_int (Int.repr 4) tint) tint])
+                             (Sset _ignore (Etempvar _ignore'2 (tptr tvoid))))
+                          (Ssequence
+                             final_loop
+                             (Sreturn None))))))))))
+  (function_body_ret_assert tvoid
+     (PROP  ()
+      LOCAL ()
+      SEP  (K_vector; `(data_at_ Tsh t_struct_SHA256state_st c);
+      `(data_block shmd
+          (intlist_to_Zlist
+             (process_msg init_registers
+                (generate_and_pad_msg
+                   (intlist_to_Zlist (map swap hashed) ++ map Int.unsigned dd))))
+          md)))).
+Proof.
+ intros Espec hashed md c shmd H md_ c_ p n cNl cNh ignore
+ hi lo dd H4 H7 H3 H3' hashed' dd' pad H0 H1 H2 H5 p0.
+ pose (hibytes := Basics.compose force_int (ZnthV tuchar (map Vint (map Int.repr (intlist_to_Zlist ([swap hi])))))).
+ pose (lobytes := Basics.compose force_int (ZnthV tuchar (map Vint (map Int.repr (intlist_to_Zlist ([swap lo])))))).
+ rewrite (split_array_at 60%Z tuchar Tsh _ (Z.of_nat CBLOCK - 8)%Z 64%Z)
+  by (change (Z.of_nat CBLOCK) with 64%Z; split; computable).
+ forward. (* cNh=c->Nh; *)
+ forward. (* (void)HOST_l2c(cNh,p); *)
+ instantiate (1:=(offset_val (Int.repr 56) (offset_val (Int.repr 40) c),
+                         Tsh, hibytes)) in (Value of witness).
+ rewrite (Z.add_comm 40).
+ entailer!.
+ destruct c; try (contradiction Pc); simpl. f_equal; rewrite Int.add_assoc; rewrite mul_repr; rewrite add_repr; reflexivity.
+ unfold hibytes.
+ symmetry; rewrite (nth_big_endian_integer 0 [hi] hi) at 1 by reflexivity.
+ f_equal; extensionality z; unfold Basics.compose.
+ f_equal; f_equal.
+ change (Z.of_nat 0 * 4)%Z with 0%Z. clear; omega.
+ pull_left   (array_at tuchar Tsh (ZnthV tuchar (map Vint dd'))
+            (Z.of_nat CBLOCK - 8) 60 (offset_val (Int.repr 40) c)) .
+ repeat rewrite sepcon_assoc.
+ apply sepcon_derives; [ | cancel_frame].
+ change 40%Z with (sizeof tuchar * 40)%Z at 1.
+ rewrite <- offset_val_array_at.
+ change (Int.repr 4) with (Int.repr (sizeof (tarray tuchar 4))).
+ rewrite memory_block_typed by reflexivity.
+ simpl_data_at.
+ change (40+56)%Z with (sizeof tuchar * (40+56))%Z.
+ rewrite <- offset_val_array_at.
+ change (40+56+4)%Z with (40+60)%Z.
+ change (40 + (Z.of_nat CBLOCK - 8))%Z with (40 + 56 + 0)%Z.
+ apply derives_refl'; apply equal_f; apply array_at_ext.
+ intros. unfold ZnthV. rewrite if_false by omega.
+ rewrite if_false by omega.
+ rewrite nth_overflow.
+ rewrite nth_overflow. auto.
+ simpl length.
+ rewrite Z2Nat.inj_sub by omega. omega.
+clear - H0 H9.
+ rewrite map_length in *.
+ change CBLOCK with 64 in H0.
+ assert (56 <= i-40)%Z by omega.
+ apply Z2Nat.inj_le in H; try omega.
+ change (Z.to_nat 56) with 56 in H; omega.
+ forward. (* p += 4; *)
+ entailer!. destruct c_; try (contradiction Pc_); apply I.
+ forward. (* cNl=c->Nl; *)
+ forward. (* (void)HOST_l2c(cNl,p); *)
+ instantiate (1:=(offset_val (Int.repr 60) (offset_val (Int.repr 40) c),
+                         Tsh, lobytes)) in (Value of witness).
+ entailer!.
+ destruct c; try (contradiction Pc); simpl.
+ f_equal; repeat rewrite Int.add_assoc; f_equal.
+ unfold lobytes.
+ symmetry; rewrite (nth_big_endian_integer 0 [lo] lo) at 1 by reflexivity.
+ f_equal; extensionality z; unfold Basics.compose.
+ f_equal; f_equal.
+ change (Z.of_nat 0 * 4)%Z with 0%Z. clear; omega.
+ pull_left   (array_at tuchar Tsh (ZnthV tuchar (map Vint dd'))
+             60 64 (offset_val (Int.repr 40) c)) .
+ repeat rewrite sepcon_assoc.
+ apply sepcon_derives; [ | cancel_frame].
+ change 40%Z with (sizeof tuchar * 40)%Z at 1.
+ rewrite <- offset_val_array_at.
+ change (Int.repr 4) with (Int.repr (sizeof (tarray tuchar 4))).
+ rewrite memory_block_typed by reflexivity.
+ simpl_data_at.
+ change (40+60)%Z with (sizeof tuchar * (40+60))%Z.
+ rewrite <- offset_val_array_at.
+ change (40+60+0)%Z with (40+60)%Z.
+ change (40 + 60+4)%Z with (40 + 64)%Z.
+ apply derives_refl'; apply equal_f; apply array_at_ext.
+ intros. unfold ZnthV. rewrite if_false by omega.
+ rewrite if_false by omega.
+ rewrite nth_overflow.
+ rewrite nth_overflow. auto.
+ simpl length.
+ rewrite Z2Nat.inj_sub by omega. omega.
+clear - H0 H10.
+ rewrite map_length in *.
+ change CBLOCK with 64 in H0.
+ assert (60 <= i-40)%Z by omega.
+ apply Z2Nat.inj_le in H; try omega.
+ change (Z.to_nat 60) with 60 in H; omega.
+ autorewrite with subst.
+ normalize.
+ forward. (* p += 4; *)
+ entailer!. destruct c_; try (contradiction Pc_); apply I.
+ forward. (*   p -= SHA_CBLOCK; *)
+ entailer!. destruct c_; try (contradiction Pc_); apply I.
+ simpl. normalize.
+ simpl force_val2. normalize.
+ replace (array_at tuchar Tsh (cVint lobytes) 0 4) with 
+     (array_at tuchar Tsh  (ZnthV tuchar
+                (map Vint (map Int.repr (intlist_to_Zlist [swap lo])))) 0 4).
+Focus 2. apply array_at_ext; intros; unfold cVint, lobytes, ZnthV, Basics.compose; if_tac; try reflexivity.
+omega.
+rewrite (nth_map' Vint Vundef Int.zero)
+ by (simpl length; apply Nat2Z.inj_lt;
+       rewrite Z2Nat.id; change (Z.of_nat 4) with 4%Z; omega).
+ reflexivity.
+ replace (array_at tuchar Tsh (cVint hibytes) 0 4) with 
+     (array_at tuchar Tsh  (ZnthV tuchar
+                (map Vint (map Int.repr (intlist_to_Zlist [swap hi])))) 0 4).
+Focus 2. apply array_at_ext; intros; unfold cVint, hibytes, ZnthV, Basics.compose; if_tac; try reflexivity.
+omega.
+rewrite (nth_map' Vint Vundef Int.zero)
+ by (simpl length; apply Nat2Z.inj_lt;
+       rewrite Z2Nat.id; change (Z.of_nat 4) with 4%Z; omega).
+ reflexivity.
+clear lobytes hibytes.
+pose (lastblock := (map Vint 
+         (dd' ++ zeros (Z.of_nat CBLOCK - 8 - Zlength dd')
+          ++  map Int.repr (intlist_to_Zlist (map swap [hi,lo]))))).
+apply semax_pre with
+ (PROP  ()
+   LOCAL 
+   (`(eq (offset_val (Int.repr 40) c)) (eval_id _p);
+   `(eq (Vint lo)) (eval_id _cNl);
+   `(eq (Vint hi)) (eval_id _cNh);
+   `(eq (Vint (Int.repr (Zlength dd')))) (eval_id _n);
+   `(eq md) (eval_id _md); `(eq c) (eval_id _c))
+   SEP 
+   (`(array_at tuchar Tsh (ZnthV tuchar lastblock) 0 64
+        (offset_val (Int.repr 40) c));
+   `(array_at tuint Tsh
+       (ZnthV tuint (map Vint (process_msg init_registers hashed'))) 0 8 c);
+   `(field_at_ Tsh t_struct_SHA256state_st _Nl c);
+   `(field_at_ Tsh t_struct_SHA256state_st _Nh c);
+   `(field_at_ Tsh t_struct_SHA256state_st _num c); 
+    K_vector;
+   `(memory_block shmd (Int.repr 32) md))).
+{unfold lastblock; clear lastblock.
+ change (intlist_to_Zlist (map swap [hi,lo])) with
+  (intlist_to_Zlist [swap hi] ++ intlist_to_Zlist [swap lo]).
+ set (hi' :=intlist_to_Zlist [swap hi]).
+ set (lo' :=  intlist_to_Zlist [swap lo]).
+ assert (Lhi: length hi' = 4) by reflexivity.
+ assert (Llo: length lo' = 4) by reflexivity.
+ assert (Hhilo: hi' = intlist_to_Zlist [swap hi] /\ lo' = intlist_to_Zlist [swap lo]) by (split; reflexivity).
+ clearbody hi' lo'.
+ entailer!.
+ destruct c_; try (contradiction Pc_); simpl;
+ f_equal; rewrite Int.sub_add_opp;
+ repeat rewrite Int.add_assoc; f_equal; reflexivity.
+ eapply (final_part5 hashed dd hashed' dd'); try eassumption.
+}
+
+
+replace lastblock with
+(map Vint (map Int.repr (intlist_to_Zlist (map swap (
+(list_drop (length hashed')
+  (generate_and_pad 
+   (intlist_to_Zlist (map swap hashed) ++ map Int.unsigned dd)
+   0))))))).
+Focus 2.
+unfold lastblock.
+f_equal.
+eapply lastblock_lemma; eassumption.
+clear lastblock.
+replace (array_at tuchar Tsh
+        (ZnthV tuchar
+           (map Vint
+              (map Int.repr
+                 (intlist_to_Zlist
+                    (map swap
+                       (list_drop (length hashed')
+                          (generate_and_pad
+                             (intlist_to_Zlist (map swap hashed) ++
+                              map Int.unsigned dd) 0))))))) 0 64)
+ with (data_block Tsh (intlist_to_Zlist
+                       (map swap
+                       (list_drop (length hashed')
+                          (generate_and_pad
+                             (intlist_to_Zlist (map swap hashed) ++
+                              map Int.unsigned dd) 0))))).
+Focus 2. {
+clear H9 H8 POSTCONDITION MORE_COMMANDS Delta p2 p3 H6 p1 p0 cNl0.
+unfold data_block, tuchars.
+f_equal.
+rewrite Zlength_correct; rewrite length_intlist_to_Zlist.
+rewrite map_length.
+rewrite list_drop_length.
+change 64%Z with (Z.of_nat (4*16)).
+f_equal. f_equal.
+admit.  (* seems fine *)
+admit.  (* seems fine *)
+} Unfocus.
+replace Delta with
+ (initialized _cNl (initialized _cNh (initialized _ignore (initialized _ignore'1 Delta_final_if1))))
+ by (simplify_Delta; reflexivity).
+eapply sha_final_part3; eassumption.
 Qed.
 
 Lemma body_SHA256_Final: semax_body Vprog Gtot f_SHA256_Final SHA256_Final_spec.
@@ -444,16 +1207,6 @@ apply exp_right with hashed.
 apply exp_right with (dd ++ [Int.repr 128]).
 apply exp_right with 0%Z.
 entailer.
-
-Lemma ltu_repr_false: forall i j, 
- (0 <= i <= Int.max_unsigned -> 
-  0 <= j <= Int.max_unsigned -> 
-  Int.ltu (Int.repr i) (Int.repr j) = false -> i>=j)%Z.
-Proof.
-intros. unfold Int.ltu in H1. if_tac in H1; inv H1.
-repeat rewrite Int.unsigned_repr in H2 by assumption.
-auto.
-Qed.
 rewrite mul_repr, sub_repr in H1; apply ltu_repr_false in H1.
 2: split; computable.
 2: assert (64 < Int.max_unsigned)%Z by computable; unfold ddlen in *;
@@ -533,4 +1286,35 @@ destruct (zlt 0 (Z.of_nat CBLOCK - 8 - Zlength dd'));
   clear - H0; admit.  (* easy *)
   clear - H0; admit.  (* easy *)
   cbv beta iota. autorewrite with subst.
-Admitted.
+  forward. (* finish the call *)
+  apply semax_pre with
+  (PROP  ()
+   LOCAL 
+   (`(eq (Vint (Int.repr (Zlength dd')))) (eval_id _n);
+   `eq (eval_id _p) (`(offset_val (Int.repr 40)) (`force_ptr (eval_id _c)));
+   `(eq md) (eval_id _md); `(eq c) (eval_id _c))
+   SEP 
+   (`(array_at tuchar Tsh (fun _ : Z => Vint Int.zero) 0
+          (Z.of_nat CBLOCK - 8 - Zlength dd')
+          (offset_val (Int.repr (Zlength dd')) (offset_val (Int.repr 40) c)));
+   `(array_at tuint Tsh
+       (ZnthV tuint (map Vint (process_msg init_registers hashed'))) 0 8 c);
+   `(field_at Tsh t_struct_SHA256state_st _Nl (Vint lo) c);
+   `(field_at Tsh t_struct_SHA256state_st _Nh (Vint hi) c);
+   `(array_at tuchar Tsh (ZnthV tuchar (map Vint dd')) 0 (Zlength dd')
+       (offset_val (Int.repr 40) c));
+   `(array_at tuchar Tsh (ZnthV tuchar (map Vint dd')) (Z.of_nat CBLOCK - 8)
+       64 (offset_val (Int.repr 40) c));
+   `(field_at_ Tsh t_struct_SHA256state_st _num c); K_vector;
+   `(memory_block shmd (Int.repr 32) md))).
+ entailer!.
+ forward.  (* p += SHA_CBLOCK-8; *)
+ entailer!.
+ simpl eval_binop. normalize.
+ unfold force_val2. simpl force_val. rewrite mul_repr, sub_repr.
+
+ replace Delta with (initialized _ignore (initialized _ignore'1 (Delta_final_if1)))
+  by (simplify_Delta; reflexivity).
+
+eapply final_part2; eassumption.
+Qed.
